Shell.lean
@@ -1,0 +1,80 @@
+import Sodium.Typography.Emulator
+
+open Lean Meta Typography Server Sodium Crypto
+
+def shell : List String := [
+  "import «Sodium».«Typography».«Frontend».«Qwerty»",
+  "open Lean Elab Meta Tactic Sodium Crypto Ethos Typography",
+  "declare_syntax_cat shell",
+  "@[reducible] def Shell := MetaM (ULift String)",
+  "elab \"#shell \" γ:term : command => do discard <| Lean.Elab.Command.elabRunMeta <| ← `(command|#eval show Shell.{1} from by exact ⟨$γ⟩)",
+]
+
+def run (uri : System.FilePath) (args : List String) (latency : Nat := 29) (delay : Nat := 31) : IO Unit := do
+  let tid ← IO.getTID
+  let shell := uri / "Shell.lean"
+  let workspace := {uri := uri.toString, name := "«shell»" : Lsp.WorkspaceFolder}
+
+  IO.FS.createDirAll uri
+  Lean.initSearchPath (← Lean.findSysroot)
+  Lean.searchPathRef.modify (uri :: ·)
+
+  let doc := {
+    uri := shell.toString
+    mod := `«Shell»
+    version := 1
+    text := FileMap.ofString <| String.intercalate "\n" args ++ "\n\n"
+    dependencyBuildMode := .once
+    : DocumentMeta
+  }
+
+  let _ ← FileWorker.setupFile doc #[] default
+
+  let config := {
+    processId? := some (Int.ofNat tid.toNat)
+    clientInfo? := some {name := "«Shell»"}
+    rootUri? := uri.toString
+    workspaceFolders? := #[workspace]
+    initializationOptions? := some {
+      editDelay? := some delay
+      hasWidgets? := true
+    }
+    capabilities := {
+      window? := some {showDocument? := some {support := false}}
+      workspace? := some {
+        applyEdit? := true
+        workspaceEdit? := some {
+          documentChanges? := true
+          changeAnnotationSupport? := some {groupsOnLabel? := true}
+          resourceOperations? := some #["create", "rename", "delete"]
+        }
+      }
+      textDocument? := some {
+        completion? := some {completionItem? := some {insertReplaceSupport? := true}}
+        inlayHint? := some {dynamicRegistration? := true, resolveSupport? := some {properties := #[]}}
+        codeAction? := none
+      }
+      lean? := some {silentDiagnosticSupport? := false}
+    }
+  }
+
+  let (ctx, st) ← FileWorker.initializeWorker doc (← IO.getStdout) (← IO.getStderr) config default
+  IO.FS.writeFile shell doc.text.source
+
+  StateRefT'.run' (s := st) <| ReaderT.run (r := ctx) <| show FileWorker.WorkerM Unit from do
+    let doc := (← get).doc
+    let hLog := (← read).hLog
+
+    let bridge : Syntax.Tactic → MetaM _
+    | `(tactic|aesop $config*) => Emulator.bridge (σ := by simp only [Encodable.encodek, implies_true, and_self]) hLog
+    | _ => Elab.throwUnsupportedSyntax
+
+    repeat match ← doc.cmdSnaps.getFinishedPrefixWithConsistentLatency latency with
+    | (snap :: _, _, true) => discard <| EIO.toBaseIO <| snap.runTermElabM doc.meta do bridge <| ← `(tactic|aesop (rule_sets := [«cautious»]))
+    | (_, some e, _) => throw e
+    | ([], _, _) | (_, _, false) => continue
+
+def main (args : List String) : IO UInt32 := do
+  let uri := (← IO.appDir) / ".." / ".."
+  run uri <| if args.length > 0 ∧ args.tail.length > 0 then args.tail else shell
+  return 0
