Sodium/Ethos.lean
@@ -1,3 +1,1 @@
 import Sodium.Ethos.Basic
-import Sodium.Ethos.Elab
-import Sodium.Ethos.Server
