Sodium/Typography/Frontend/Qwerty.lean
@@ -1,0 +1,966 @@
+import Sodium.Typography.Emulator
+
+open Lean Parser Elab Meta Term Tactic PrettyPrinter
+
+namespace Typography
+
+variable {σ}
+
+declare_syntax_cat grapheme
+declare_syntax_cat terminal
+
+syntax (name := terminal) &"\n" : terminal
+
+syntax (name := a) "a" : grapheme
+syntax (name := b) "b" : grapheme
+syntax (name := c) "c" : grapheme
+syntax (name := d) "d" : grapheme
+syntax (name := e) "e" : grapheme
+syntax (name := f) "f" : grapheme
+syntax (name := g) "g" : grapheme
+syntax (name := h) "h" : grapheme
+syntax (name := i) "i" : grapheme
+syntax (name := j) "j" : grapheme
+syntax (name := k) "k" : grapheme
+syntax (name := l) "l" : grapheme
+syntax (name := m) "m" : grapheme
+syntax (name := n) "n" : grapheme
+syntax (name := o) "o" : grapheme
+syntax (name := p) "p" : grapheme
+syntax (name := q) "q" : grapheme
+syntax (name := r) "r" : grapheme
+syntax (name := s) "s" : grapheme
+syntax (name := t) "t" : grapheme
+syntax (name := u) "u" : grapheme
+syntax (name := v) "v" : grapheme
+syntax (name := w) "w" : grapheme
+syntax (name := x) "x" : grapheme
+syntax (name := y) "y" : grapheme
+syntax (name := z) "z" : grapheme
+syntax (name := A) "A" : grapheme
+syntax (name := B) "B" : grapheme
+syntax (name := C) "C" : grapheme
+syntax (name := D) "D" : grapheme
+syntax (name := E) "E" : grapheme
+syntax (name := F) "F" : grapheme
+syntax (name := G) "G" : grapheme
+syntax (name := H) "H" : grapheme
+syntax (name := I) "I" : grapheme
+syntax (name := J) "J" : grapheme
+syntax (name := K) "K" : grapheme
+syntax (name := L) "L" : grapheme
+syntax (name := M) "M" : grapheme
+syntax (name := N) "N" : grapheme
+syntax (name := O) "O" : grapheme
+syntax (name := P) "P" : grapheme
+syntax (name := Q) "Q" : grapheme
+syntax (name := R) "R" : grapheme
+syntax (name := S) "S" : grapheme
+syntax (name := T) "T" : grapheme
+syntax (name := U) "U" : grapheme
+syntax (name := V) "V" : grapheme
+syntax (name := W) "W" : grapheme
+syntax (name := X) "X" : grapheme
+syntax (name := Y) "Y" : grapheme
+syntax (name := Z) "Z" : grapheme
+syntax (name := zero) &"0" : grapheme
+syntax (name := one) &"1" : grapheme
+syntax (name := two) &"2" : grapheme
+syntax (name := three) &"3" : grapheme
+syntax (name := four) &"4" : grapheme
+syntax (name := five) &"5" : grapheme
+syntax (name := six) &"6" : grapheme
+syntax (name := seven) &"7" : grapheme
+syntax (name := eight) &"8" : grapheme
+syntax (name := nine) &"9" : grapheme
+syntax (name := exclamation) &"!" : grapheme
+syntax (name := sign) &"@" : grapheme
+syntax (name := hash) &"#" : grapheme
+syntax (name := dollar) &"$" : grapheme
+syntax (name := percent) &"%" : grapheme
+syntax (name := caret) &"^" : grapheme
+syntax (name := ampersand) &"&" : grapheme
+syntax (name := asterisk) &"*" : grapheme
+syntax (name := lparen) &"(" : grapheme
+syntax (name := rparen) &")" : grapheme
+syntax (name := hyphen) &"-" : grapheme
+syntax (name := underscore) &"_" : grapheme
+syntax (name := equals) &"=" : grapheme
+syntax (name := plus) &"+" : grapheme
+syntax (name := lbracket) &"[" : grapheme
+syntax (name := rbracket) &"]" : grapheme
+syntax (name := lbrace) &"{" : grapheme
+syntax (name := rbrace) &"}" : grapheme
+syntax (name := slash) &"\\" : grapheme
+syntax (name := pipe) &"|" : grapheme
+syntax (name := semicolon) &";" : grapheme
+syntax (name := colon) &":" : grapheme
+syntax (name := apostrophe) &"'" : grapheme
+syntax (name := quote) &"\"" : grapheme
+syntax (name := comma) &"," : grapheme
+syntax (name := period) &"." : grapheme
+syntax (name := langle) &"<" : grapheme
+syntax (name := rangle) &">" : grapheme
+syntax (name := divide) &"/" : grapheme
+syntax (name := question) &"?" : grapheme
+syntax (name := grave) &"`" : grapheme
+syntax (name := tilde) &"~" : grapheme
+syntax (name := space) &" " : grapheme
+
+syntax (name := leader) "leader% " (grapheme)? : term
+syntax (name := done) "done% " (terminal)? : term
+
+def Terminal := TSyntax `terminal
+
+@[reducible]
+def Carriage : Terminal := ⟨mkNode ``terminal #[mkAtom "\n"]⟩
+
+instance : Inhabited Terminal := ⟨Carriage⟩
+instance : Encodable Terminal := by unfold Terminal; infer_instance
+
+def newline : Terminal → TermElabM Char
+| stx => match stx.raw.getKind with
+  | ``terminal => pure '\n'
+  | _ => throwUnsupportedSyntax
+
+@[reducible]
+def Grapheme := TSyntax `grapheme
+
+@[reducible]
+def Space : Grapheme := ⟨mkNode ``space #[mkAtom " "]⟩
+
+instance : Inhabited Grapheme := ⟨Space⟩
+instance : Encodable Grapheme := by unfold Grapheme; infer_instance
+
+def parse : Grapheme → TermElabM Char
+| `(grapheme|a) => pure 'a'
+| `(grapheme|b) => pure 'b'
+| `(grapheme|c) => pure 'c'
+| `(grapheme|d) => pure 'd'
+| `(grapheme|e) => pure 'e'
+| `(grapheme|f) => pure 'f'
+| `(grapheme|g) => pure 'g'
+| `(grapheme|h) => pure 'h'
+| `(grapheme|i) => pure 'i'
+| `(grapheme|j) => pure 'j'
+| `(grapheme|k) => pure 'k'
+| `(grapheme|l) => pure 'l'
+| `(grapheme|m) => pure 'm'
+| `(grapheme|n) => pure 'n'
+| `(grapheme|o) => pure 'o'
+| `(grapheme|p) => pure 'p'
+| `(grapheme|q) => pure 'q'
+| `(grapheme|r) => pure 'r'
+| `(grapheme|s) => pure 's'
+| `(grapheme|t) => pure 't'
+| `(grapheme|u) => pure 'u'
+| `(grapheme|v) => pure 'v'
+| `(grapheme|w) => pure 'w'
+| `(grapheme|x) => pure 'x'
+| `(grapheme|y) => pure 'y'
+| `(grapheme|z) => pure 'z'
+| `(grapheme|A) => pure 'A'
+| `(grapheme|B) => pure 'B'
+| `(grapheme|C) => pure 'C'
+| `(grapheme|D) => pure 'D'
+| `(grapheme|E) => pure 'E'
+| `(grapheme|F) => pure 'F'
+| `(grapheme|G) => pure 'G'
+| `(grapheme|H) => pure 'H'
+| `(grapheme|I) => pure 'I'
+| `(grapheme|J) => pure 'J'
+| `(grapheme|K) => pure 'K'
+| `(grapheme|L) => pure 'L'
+| `(grapheme|M) => pure 'M'
+| `(grapheme|N) => pure 'N'
+| `(grapheme|O) => pure 'O'
+| `(grapheme|P) => pure 'P'
+| `(grapheme|Q) => pure 'Q'
+| `(grapheme|R) => pure 'R'
+| `(grapheme|S) => pure 'S'
+| `(grapheme|T) => pure 'T'
+| `(grapheme|U) => pure 'U'
+| `(grapheme|V) => pure 'V'
+| `(grapheme|W) => pure 'W'
+| `(grapheme|X) => pure 'X'
+| `(grapheme|Y) => pure 'Y'
+| `(grapheme|Z) => pure 'Z'
+| stx => match stx.raw.getKind with
+  | ``space => pure ' '
+  | ``zero => pure '0'
+  | ``one => pure '1'
+  | ``two => pure '2'
+  | ``three => pure '3'
+  | ``four => pure '4'
+  | ``five => pure '5'
+  | ``six => pure '6'
+  | ``seven => pure '7'
+  | ``eight => pure '8'
+  | ``nine => pure '9'
+  | ``exclamation => pure '!'
+  | ``sign => pure '@'
+  | ``hash => pure '#'
+  | ``dollar => pure '$'
+  | ``percent => pure '%'
+  | ``caret => pure '^'
+  | ``ampersand => pure '&'
+  | ``asterisk => pure '*'
+  | ``lparen => pure '('
+  | ``rparen => pure ')'
+  | ``hyphen => pure '-'
+  | ``underscore => pure '_'
+  | ``equals => pure '='
+  | ``plus => pure '+'
+  | ``lbracket => pure '['
+  | ``rbracket => pure ']'
+  | ``lbrace => pure '{'
+  | ``rbrace => pure '}'
+  | ``slash => pure '\\'
+  | ``pipe => pure '|'
+  | ``semicolon => pure ';'
+  | ``colon => pure ':'
+  | ``apostrophe => pure '\''
+  | ``quote => pure '"'
+  | ``comma => pure ','
+  | ``period => pure '.'
+  | ``langle => pure '<'
+  | ``rangle => pure '>'
+  | ``divide => pure '/'
+  | ``question => pure '?'
+  | ``grave => pure '`'
+  | ``tilde => pure '~'
+  | _ => throwUnsupportedSyntax
+
+elab "leader% " γ:(grapheme)? : tactic => do
+  let γ ← parse <| γ.getD default
+  let γ := Syntax.mkCharLit γ
+  evalTactic <| ← `(tactic|exact ⟨$γ⟩)
+
+elab "done%" : tactic => do
+  let γ ← newline default
+  let γ := Syntax.mkCharLit γ
+  evalTactic <| ← `(tactic|exact ⟨$γ⟩)
+
+section Digits
+
+abbrev Zero : Grapheme := ⟨mkNode ``zero #[mkAtom "0"]⟩
+abbrev One : Grapheme := ⟨mkNode ``one #[mkAtom "1"]⟩
+abbrev Two : Grapheme := ⟨mkNode ``two #[mkAtom "2"]⟩
+abbrev Three : Grapheme := ⟨mkNode ``three #[mkAtom "3"]⟩
+abbrev Four : Grapheme := ⟨mkNode ``four #[mkAtom "4"]⟩
+abbrev Five : Grapheme := ⟨mkNode ``five #[mkAtom "5"]⟩
+abbrev Six : Grapheme := ⟨mkNode ``six #[mkAtom "6"]⟩
+abbrev Seven : Grapheme := ⟨mkNode ``seven #[mkAtom "7"]⟩
+abbrev Eight : Grapheme := ⟨mkNode ``eight #[mkAtom "8"]⟩
+abbrev Nine : Grapheme := ⟨mkNode ``nine #[mkAtom "9"]⟩
+
+end Digits
+
+section Symbols
+
+abbrev Exclamation : Grapheme := ⟨mkNode ``exclamation #[mkAtom "!"]⟩
+abbrev Sign : Grapheme := ⟨mkNode ``sign #[mkAtom "@"]⟩
+abbrev Hash : Grapheme := ⟨mkNode ``hash #[mkAtom "#"]⟩
+abbrev Dollar : Grapheme := ⟨mkNode ``dollar #[mkAtom "$"]⟩
+abbrev Percent : Grapheme := ⟨mkNode ``percent #[mkAtom "%"]⟩
+abbrev Caret : Grapheme := ⟨mkNode ``caret #[mkAtom "^"]⟩
+abbrev Ampersand : Grapheme := ⟨mkNode ``ampersand #[mkAtom "&"]⟩
+abbrev Asterisk : Grapheme := ⟨mkNode ``asterisk #[mkAtom "*"]⟩
+abbrev Lparen : Grapheme := ⟨mkNode ``lparen #[mkAtom "("]⟩
+abbrev Rparen : Grapheme := ⟨mkNode ``rparen #[mkAtom ")"]⟩
+abbrev Hyphen : Grapheme := ⟨mkNode ``hyphen #[mkAtom "-"]⟩
+abbrev Underscore : Grapheme := ⟨mkNode ``underscore #[mkAtom "_"]⟩
+abbrev Equals : Grapheme := ⟨mkNode ``equals #[mkAtom "="]⟩
+abbrev Plus : Grapheme := ⟨mkNode ``plus #[mkAtom "+"]⟩
+abbrev Lbracket : Grapheme := ⟨mkNode ``lbracket #[mkAtom "["]⟩
+abbrev Rbracket : Grapheme := ⟨mkNode ``rbracket #[mkAtom "]"]⟩
+abbrev Lbrace : Grapheme := ⟨mkNode ``lbrace #[mkAtom "{"]⟩
+abbrev Rbrace : Grapheme := ⟨mkNode ``rbrace #[mkAtom "}"]⟩
+abbrev Slash : Grapheme := ⟨mkNode ``slash #[mkAtom "\\"]⟩
+abbrev Pipe : Grapheme := ⟨mkNode ``pipe #[mkAtom "|"]⟩
+abbrev Semicolon : Grapheme := ⟨mkNode ``semicolon #[mkAtom ";"]⟩
+abbrev Colon : Grapheme := ⟨mkNode ``colon #[mkAtom ":"]⟩
+abbrev Apostrophe : Grapheme := ⟨mkNode ``apostrophe #[mkAtom "'"]⟩
+abbrev Quote : Grapheme := ⟨mkNode ``quote #[mkAtom "\""]⟩
+abbrev Comma : Grapheme := ⟨mkNode ``comma #[mkAtom ","]⟩
+abbrev Period : Grapheme := ⟨mkNode ``period #[mkAtom "."]⟩
+abbrev Langle : Grapheme := ⟨mkNode ``langle #[mkAtom "<"]⟩
+abbrev Rangle : Grapheme := ⟨mkNode ``rangle #[mkAtom ">"]⟩
+abbrev Divide : Grapheme := ⟨mkNode ``divide #[mkAtom "/"]⟩
+abbrev Question : Grapheme := ⟨mkNode ``question #[mkAtom "?"]⟩
+abbrev Grave : Grapheme := ⟨mkNode ``grave #[mkAtom "`"]⟩
+abbrev Tilde : Grapheme := ⟨mkNode ``tilde #[mkAtom "~"]⟩
+
+end Symbols
+
+section Alphabet
+
+abbrev alpha : Grapheme := ⟨mkNode ``«a» #[mkAtom "a"]⟩
+abbrev beta : Grapheme := ⟨mkNode ``«b» #[mkAtom "b"]⟩
+abbrev gamma : Grapheme := ⟨mkNode ``«c» #[mkAtom "c"]⟩
+abbrev delta : Grapheme := ⟨mkNode ``«d» #[mkAtom "d"]⟩
+abbrev epsilon : Grapheme := ⟨mkNode ``«e» #[mkAtom "e"]⟩
+abbrev zeta : Grapheme := ⟨mkNode ``«f» #[mkAtom "f"]⟩
+abbrev eta : Grapheme := ⟨mkNode ``«g» #[mkAtom "g"]⟩
+abbrev theta : Grapheme := ⟨mkNode ``«h» #[mkAtom "h"]⟩
+abbrev iota : Grapheme := ⟨mkNode ``«i» #[mkAtom "i"]⟩
+abbrev kappa : Grapheme := ⟨mkNode ``«j» #[mkAtom "j"]⟩
+abbrev lambda : Grapheme := ⟨mkNode ``«k» #[mkAtom "k"]⟩
+abbrev mu : Grapheme := ⟨mkNode ``«l» #[mkAtom "l"]⟩
+abbrev nu : Grapheme := ⟨mkNode ``«m» #[mkAtom "m"]⟩
+abbrev xi : Grapheme := ⟨mkNode ``«n» #[mkAtom "n"]⟩
+abbrev omicron : Grapheme := ⟨mkNode ``«o» #[mkAtom "o"]⟩
+abbrev pi : Grapheme := ⟨mkNode ``«p» #[mkAtom "p"]⟩
+abbrev rho : Grapheme := ⟨mkNode ``«q» #[mkAtom "q"]⟩
+abbrev sigma : Grapheme := ⟨mkNode ``«r» #[mkAtom "r"]⟩
+abbrev tau : Grapheme := ⟨mkNode ``«s» #[mkAtom "s"]⟩
+abbrev upsilon : Grapheme := ⟨mkNode ``«t» #[mkAtom "t"]⟩
+abbrev phi : Grapheme := ⟨mkNode ``«u» #[mkAtom "u"]⟩
+abbrev chi : Grapheme := ⟨mkNode ``«v» #[mkAtom "v"]⟩
+abbrev psi : Grapheme := ⟨mkNode ``«w» #[mkAtom "w"]⟩
+abbrev omega : Grapheme := ⟨mkNode ``«x» #[mkAtom "x"]⟩
+abbrev why : Grapheme := ⟨mkNode ``«y» #[mkAtom "y"]⟩
+abbrev zed : Grapheme := ⟨mkNode ``«z» #[mkAtom "z"]⟩
+
+abbrev Alpha : Grapheme := ⟨mkNode ``«A» #[mkAtom "A"]⟩
+abbrev Beta : Grapheme := ⟨mkNode ``«B» #[mkAtom "B"]⟩
+abbrev Gamma : Grapheme := ⟨mkNode ``«C» #[mkAtom "C"]⟩
+abbrev Delta : Grapheme := ⟨mkNode ``«D» #[mkAtom "D"]⟩
+abbrev Epsilon : Grapheme := ⟨mkNode ``«E» #[mkAtom "E"]⟩
+abbrev Zeta : Grapheme := ⟨mkNode ``«F» #[mkAtom "F"]⟩
+abbrev Eta : Grapheme := ⟨mkNode ``«G» #[mkAtom "G"]⟩
+abbrev Theta : Grapheme := ⟨mkNode ``«H» #[mkAtom "H"]⟩
+abbrev Iota : Grapheme := ⟨mkNode ``«I» #[mkAtom "I"]⟩
+abbrev Kappa : Grapheme := ⟨mkNode ``«J» #[mkAtom "J"]⟩
+abbrev Lambda : Grapheme := ⟨mkNode ``«K» #[mkAtom "K"]⟩
+abbrev Mu : Grapheme := ⟨mkNode ``«L» #[mkAtom "L"]⟩
+abbrev Nu : Grapheme := ⟨mkNode ``«M» #[mkAtom "M"]⟩
+abbrev Xi : Grapheme := ⟨mkNode ``«N» #[mkAtom "N"]⟩
+abbrev Omicron : Grapheme := ⟨mkNode ``«O» #[mkAtom "O"]⟩
+abbrev Pi : Grapheme := ⟨mkNode ``«P» #[mkAtom "P"]⟩
+abbrev Rho : Grapheme := ⟨mkNode ``«Q» #[mkAtom "Q"]⟩
+abbrev Sigma : Grapheme := ⟨mkNode ``«R» #[mkAtom "R"]⟩
+abbrev Tau : Grapheme := ⟨mkNode ``«S» #[mkAtom "S"]⟩
+abbrev Upsilon : Grapheme := ⟨mkNode ``«T» #[mkAtom "T"]⟩
+abbrev Phi : Grapheme := ⟨mkNode ``«U» #[mkAtom "U"]⟩
+abbrev Chi : Grapheme := ⟨mkNode ``«V» #[mkAtom "V"]⟩
+abbrev Psi : Grapheme := ⟨mkNode ``«W» #[mkAtom "W"]⟩
+abbrev Omega : Grapheme := ⟨mkNode ``«X» #[mkAtom "X"]⟩
+abbrev Why : Grapheme := ⟨mkNode ``«Y» #[mkAtom "Y"]⟩
+abbrev Zed : Grapheme := ⟨mkNode ``«Z» #[mkAtom "Z"]⟩
+
+end Alphabet
+
+abbrev Symbol (γ : Grapheme) : TermElabM Syntax.Tactic := `(tactic|leader% $γ)
+abbrev Return : TermElabM Syntax.Tactic := `(tactic|done%)
+
+def Key := Option (Grapheme ⊕ Terminal)
+
+namespace Key
+
+notation "spin%" => some (Sum.inr («α» := «Grapheme») default)
+notation "turn% " γ => some (Sum.inl («α» := «Grapheme») («β» := «Terminal») γ)
+
+@[simp] theorem spin_rfl : spin% = some (Sum.inr Carriage) := by rfl
+@[simp] theorem turn_rfl : ∀ γ, (turn% γ) = some (Sum.inl γ) := by intro; rfl
+
+@[coe]
+def toPoint : Key → Point
+| turn% γ => point% ⟨γ.raw⟩
+| spin% => bot%
+| _ => none
+
+deriving instance TypeName for Key
+instance : Inhabited Key := ⟨spin%⟩
+instance : Encodable Key := by unfold Key; infer_instance
+instance : Coe Key Point := ⟨toPoint⟩
+
+def mk : Char → Key
+| 'a' => turn% alpha
+| 'b' => turn% beta
+| 'c' => turn% gamma
+| 'd' => turn% delta
+| 'e' => turn% epsilon
+| 'f' => turn% zeta
+| 'g' => turn% eta
+| 'h' => turn% theta
+| 'i' => turn% iota
+| 'j' => turn% kappa
+| 'k' => turn% lambda
+| 'l' => turn% mu
+| 'm' => turn% nu
+| 'n' => turn% xi
+| 'o' => turn% omicron
+| 'p' => turn% pi
+| 'q' => turn% rho
+| 'r' => turn% sigma
+| 's' => turn% tau
+| 't' => turn% upsilon
+| 'u' => turn% phi
+| 'v' => turn% chi
+| 'w' => turn% psi
+| 'x' => turn% omega
+| 'y' => turn% why
+| 'z' => turn% zed
+| 'A' => turn% Alpha
+| 'B' => turn% Beta
+| 'C' => turn% Gamma
+| 'D' => turn% Delta
+| 'E' => turn% Epsilon
+| 'F' => turn% Zeta
+| 'G' => turn% Eta
+| 'H' => turn% Theta
+| 'I' => turn% Iota
+| 'J' => turn% Kappa
+| 'K' => turn% Lambda
+| 'L' => turn% Mu
+| 'M' => turn% Nu
+| 'N' => turn% Xi
+| 'O' => turn% Omicron
+| 'P' => turn% Pi
+| 'Q' => turn% Rho
+| 'R' => turn% Sigma
+| 'S' => turn% Tau
+| 'T' => turn% Upsilon
+| 'U' => turn% Phi
+| 'V' => turn% Chi
+| 'W' => turn% Psi
+| 'X' => turn% Omega
+| 'Y' => turn% Why
+| 'Z' => turn% Zed
+| '0' => turn% Zero
+| '1' => turn% One
+| '2' => turn% Two
+| '3' => turn% Three
+| '4' => turn% Four
+| '5' => turn% Five
+| '6' => turn% Six
+| '7' => turn% Seven
+| '8' => turn% Eight
+| '9' => turn% Nine
+| '!' => turn% Exclamation
+| '@' => turn% Sign
+| '#' => turn% Hash
+| '$' => turn% Dollar
+| '%' => turn% Percent
+| '^' => turn% Caret
+| '&' => turn% Ampersand
+| '*' => turn% Asterisk
+| '(' => turn% Lparen
+| ')' => turn% Rparen
+| '-' => turn% Hyphen
+| '_' => turn% Underscore
+| '=' => turn% Equals
+| '+' => turn% Plus
+| '[' => turn% Lbracket
+| ']' => turn% Rbracket
+| '{' => turn% Lbrace
+| '}' => turn% Rbrace
+| '|' => turn% Pipe
+| ';' => turn% Semicolon
+| ':' => turn% Colon
+| '"' => turn% Quote
+| ',' => turn% Comma
+| '.' => turn% Period
+| '<' => turn% Langle
+| '>' => turn% Rangle
+| '/' => turn% Divide
+| '?' => turn% Question
+| '`' => turn% Grave
+| '~' => turn% Tilde
+| ' ' => turn% Space
+| '\\' => turn% Slash
+| '\'' => turn% Apostrophe
+| '\n' => spin%
+| _ => none
+
+def ofByteArray : ByteArray → Array Key
+| ⟨γ⟩ => γ.map (Key.mk ∘ Char.ofUInt8)
+
+def ofFin : Fin 97 → Key
+| 0 => turn% Space
+| 1 => turn% Exclamation
+| 2 => turn% Quote
+| 3 => turn% Hash
+| 4 => turn% Dollar
+| 5 => turn% Percent
+| 6 => turn% Ampersand
+| 7 => turn% Apostrophe
+| 8 => turn% Lparen
+| 9 => turn% Rparen
+| 10 => turn% Asterisk
+| 11 => turn% Plus
+| 12 => turn% Comma
+| 13 => turn% Hyphen
+| 14 => turn% Period
+| 15 => turn% Divide
+| 16 => turn% Zero
+| 17 => turn% One
+| 18 => turn% Two
+| 19 => turn% Three
+| 20 => turn% Four
+| 21 => turn% Five
+| 22 => turn% Six
+| 23 => turn% Seven
+| 24 => turn% Eight
+| 25 => turn% Nine
+| 26 => turn% Colon
+| 27 => turn% Semicolon
+| 28 => turn% Langle
+| 29 => turn% Equals
+| 30 => turn% Rangle
+| 31 => turn% Question
+| 32 => turn% Sign
+| 33 => turn% Alpha
+| 34 => turn% Beta
+| 35 => turn% Gamma
+| 36 => turn% Delta
+| 37 => turn% Epsilon
+| 38 => turn% Zeta
+| 39 => turn% Eta
+| 40 => turn% Theta
+| 41 => turn% Iota
+| 42 => turn% Kappa
+| 43 => turn% Lambda
+| 44 => turn% Mu
+| 45 => turn% Nu
+| 46 => turn% Xi
+| 47 => turn% Omicron
+| 48 => turn% Pi
+| 49 => turn% Rho
+| 50 => turn% Sigma
+| 51 => turn% Tau
+| 52 => turn% Upsilon
+| 53 => turn% Phi
+| 54 => turn% Chi
+| 55 => turn% Psi
+| 56 => turn% Omega
+| 57 => turn% Why
+| 58 => turn% Zed
+| 59 => turn% Lbracket
+| 60 => turn% Slash
+| 61 => turn% Rbracket
+| 62 => turn% Caret
+| 63 => turn% Underscore
+| 64 => turn% Grave
+| 65 => turn% alpha
+| 66 => turn% beta
+| 67 => turn% gamma
+| 68 => turn% delta
+| 69 => turn% epsilon
+| 70 => turn% zeta
+| 71 => turn% eta
+| 72 => turn% theta
+| 73 => turn% iota
+| 74 => turn% kappa
+| 75 => turn% lambda
+| 76 => turn% mu
+| 77 => turn% nu
+| 78 => turn% xi
+| 79 => turn% omicron
+| 80 => turn% pi
+| 81 => turn% rho
+| 82 => turn% sigma
+| 83 => turn% tau
+| 84 => turn% upsilon
+| 85 => turn% phi
+| 86 => turn% chi
+| 87 => turn% psi
+| 88 => turn% omega
+| 89 => turn% why
+| 90 => turn% zed
+| 91 => turn% Lbrace
+| 92 => turn% Pipe
+| 93 => turn% Rbrace
+| 94 => turn% Tilde
+| 95 => spin%
+| _ => none
+
+def toFin : Key → Fin 97
+| turn% ⟨.node _ ``space _⟩ => 0
+| turn% ⟨.node _ ``exclamation _⟩ => 1
+| turn% ⟨.node _ ``quote _⟩ => 2
+| turn% ⟨.node _ ``hash _⟩ => 3
+| turn% ⟨.node _ ``dollar _⟩ => 4
+| turn% ⟨.node _ ``percent _⟩ => 5
+| turn% ⟨.node _ ``ampersand _⟩ => 6
+| turn% ⟨.node _ ``apostrophe _⟩ => 7
+| turn% ⟨.node _ ``lparen _⟩ => 8
+| turn% ⟨.node _ ``rparen _⟩ => 9
+| turn% ⟨.node _ ``asterisk _⟩ => 10
+| turn% ⟨.node _ ``plus _⟩ => 11
+| turn% ⟨.node _ ``comma _⟩ => 12
+| turn% ⟨.node _ ``hyphen _⟩ => 13
+| turn% ⟨.node _ ``period _⟩ => 14
+| turn% ⟨.node _ ``divide _⟩ => 15
+| turn% ⟨.node _ ``zero _⟩ => 16
+| turn% ⟨.node _ ``one _⟩ => 17
+| turn% ⟨.node _ ``two _⟩ => 18
+| turn% ⟨.node _ ``three _⟩ => 19
+| turn% ⟨.node _ ``four _⟩ => 20
+| turn% ⟨.node _ ``five _⟩ => 21
+| turn% ⟨.node _ ``six _⟩ => 22
+| turn% ⟨.node _ ``seven _⟩ => 23
+| turn% ⟨.node _ ``eight _⟩ => 24
+| turn% ⟨.node _ ``nine _⟩ => 25
+| turn% ⟨.node _ ``colon _⟩ => 26
+| turn% ⟨.node _ ``semicolon _⟩ => 27
+| turn% ⟨.node _ ``langle _⟩ => 28
+| turn% ⟨.node _ ``equals _⟩ => 29
+| turn% ⟨.node _ ``rangle _⟩ => 30
+| turn% ⟨.node _ ``question _⟩ => 31
+| turn% ⟨.node _ ``sign _⟩ => 32
+| turn% ⟨.node _ ``«A» _⟩ => 33
+| turn% ⟨.node _ ``«B» _⟩ => 34
+| turn% ⟨.node _ ``«C» _⟩ => 35
+| turn% ⟨.node _ ``«D» _⟩ => 36
+| turn% ⟨.node _ ``«E» _⟩ => 37
+| turn% ⟨.node _ ``«F» _⟩ => 38
+| turn% ⟨.node _ ``«G» _⟩ => 39
+| turn% ⟨.node _ ``«H» _⟩ => 40
+| turn% ⟨.node _ ``«I» _⟩ => 41
+| turn% ⟨.node _ ``«J» _⟩ => 42
+| turn% ⟨.node _ ``«K» _⟩ => 43
+| turn% ⟨.node _ ``«L» _⟩ => 44
+| turn% ⟨.node _ ``«M» _⟩ => 45
+| turn% ⟨.node _ ``«N» _⟩ => 46
+| turn% ⟨.node _ ``«O» _⟩ => 47
+| turn% ⟨.node _ ``«P» _⟩ => 48
+| turn% ⟨.node _ ``«Q» _⟩ => 49
+| turn% ⟨.node _ ``«R» _⟩ => 50
+| turn% ⟨.node _ ``«S» _⟩ => 51
+| turn% ⟨.node _ ``«T» _⟩ => 52
+| turn% ⟨.node _ ``«U» _⟩ => 53
+| turn% ⟨.node _ ``«V» _⟩ => 54
+| turn% ⟨.node _ ``«W» _⟩ => 55
+| turn% ⟨.node _ ``«X» _⟩ => 56
+| turn% ⟨.node _ ``«Y» _⟩ => 57
+| turn% ⟨.node _ ``«Z» _⟩ => 58
+| turn% ⟨.node _ ``lbracket _⟩ => 59
+| turn% ⟨.node _ ``slash _⟩ => 60
+| turn% ⟨.node _ ``rbracket _⟩ => 61
+| turn% ⟨.node _ ``caret _⟩ => 62
+| turn% ⟨.node _ ``underscore _⟩ => 63
+| turn% ⟨.node _ ``grave _⟩ => 64
+| turn% ⟨.node _ ``«a» _⟩ => 65
+| turn% ⟨.node _ ``«b» _⟩ => 66
+| turn% ⟨.node _ ``«c» _⟩ => 67
+| turn% ⟨.node _ ``«d» _⟩ => 68
+| turn% ⟨.node _ ``«e» _⟩ => 69
+| turn% ⟨.node _ ``«f» _⟩ => 70
+| turn% ⟨.node _ ``«g» _⟩ => 71
+| turn% ⟨.node _ ``«h» _⟩ => 72
+| turn% ⟨.node _ ``«i» _⟩ => 73
+| turn% ⟨.node _ ``«j» _⟩ => 74
+| turn% ⟨.node _ ``«k» _⟩ => 75
+| turn% ⟨.node _ ``«l» _⟩ => 76
+| turn% ⟨.node _ ``«m» _⟩ => 77
+| turn% ⟨.node _ ``«n» _⟩ => 78
+| turn% ⟨.node _ ``«o» _⟩ => 79
+| turn% ⟨.node _ ``«p» _⟩ => 80
+| turn% ⟨.node _ ``«q» _⟩ => 81
+| turn% ⟨.node _ ``«r» _⟩ => 82
+| turn% ⟨.node _ ``«s» _⟩ => 83
+| turn% ⟨.node _ ``«t» _⟩ => 84
+| turn% ⟨.node _ ``«u» _⟩ => 85
+| turn% ⟨.node _ ``«v» _⟩ => 86
+| turn% ⟨.node _ ``«w» _⟩ => 87
+| turn% ⟨.node _ ``«x» _⟩ => 88
+| turn% ⟨.node _ ``«y» _⟩ => 89
+| turn% ⟨.node _ ``«z» _⟩ => 90
+| turn% ⟨.node _ ``lbrace _⟩ => 91
+| turn% ⟨.node _ ``pipe _⟩ => 92
+| turn% ⟨.node _ ``rbrace _⟩ => 93
+| turn% ⟨.node _ ``tilde _⟩ => 94
+| spin% => 95
+| _ => 96
+
+open Sodium Crypto Ethos in
+def quantize {τ : Sodium σ} (scope : ScopeName := .global) : Key → CryptoM τ Observable
+| turn% γ => do Observable.new <| ← `(tactic|leader% $γ)
+| spin% => do Observable.new <| ← `(tactic|done%)
+| _ => Observable.pointer scope
+
+end Key
+
+def Shape.pull : Shape → Key
+| some (some γ) => Key.mk γ
+| some none => spin%
+| _ => none
+
+def Shape.push : Key → Shape
+| turn% ⟨.node _ ``space _⟩ => shape% ' '
+| turn% ⟨.node _ ``exclamation _⟩ => shape% '!'
+| turn% ⟨.node _ ``quote _⟩ => shape% '"'
+| turn% ⟨.node _ ``hash _⟩ => shape% '#'
+| turn% ⟨.node _ ``dollar _⟩ => shape% '$'
+| turn% ⟨.node _ ``percent _⟩ => shape% '%'
+| turn% ⟨.node _ ``ampersand _⟩ => shape% '&'
+| turn% ⟨.node _ ``apostrophe _⟩ => shape% '\''
+| turn% ⟨.node _ ``lparen _⟩ => shape% '('
+| turn% ⟨.node _ ``rparen _⟩ => shape% ')'
+| turn% ⟨.node _ ``asterisk _⟩ => shape% '*'
+| turn% ⟨.node _ ``plus _⟩ => shape% '+'
+| turn% ⟨.node _ ``comma _⟩ => shape% ','
+| turn% ⟨.node _ ``hyphen _⟩ => shape% '-'
+| turn% ⟨.node _ ``period _⟩ => shape% '.'
+| turn% ⟨.node _ ``divide _⟩ => shape% '/'
+| turn% ⟨.node _ ``zero _⟩ => shape% '0'
+| turn% ⟨.node _ ``one _⟩ => shape% '1'
+| turn% ⟨.node _ ``two _⟩ => shape% '2'
+| turn% ⟨.node _ ``three _⟩ => shape% '3'
+| turn% ⟨.node _ ``four _⟩ => shape% '4'
+| turn% ⟨.node _ ``five _⟩ => shape% '5'
+| turn% ⟨.node _ ``six _⟩ => shape% '6'
+| turn% ⟨.node _ ``seven _⟩ => shape% '7'
+| turn% ⟨.node _ ``eight _⟩ => shape% '8'
+| turn% ⟨.node _ ``nine _⟩ => shape% '9'
+| turn% ⟨.node _ ``colon _⟩ => shape% ':'
+| turn% ⟨.node _ ``semicolon _⟩ => shape% ';'
+| turn% ⟨.node _ ``langle _⟩ => shape% '<'
+| turn% ⟨.node _ ``equals _⟩ => shape% '='
+| turn% ⟨.node _ ``rangle _⟩ => shape% '>'
+| turn% ⟨.node _ ``question _⟩ => shape% '?'
+| turn% ⟨.node _ ``sign _⟩ => shape% '@'
+| turn% ⟨.node _ ``«A» _⟩ => shape% 'A'
+| turn% ⟨.node _ ``«B» _⟩ => shape% 'B'
+| turn% ⟨.node _ ``«C» _⟩ => shape% 'C'
+| turn% ⟨.node _ ``«D» _⟩ => shape% 'D'
+| turn% ⟨.node _ ``«E» _⟩ => shape% 'E'
+| turn% ⟨.node _ ``«F» _⟩ => shape% 'F'
+| turn% ⟨.node _ ``«G» _⟩ => shape% 'G'
+| turn% ⟨.node _ ``«H» _⟩ => shape% 'H'
+| turn% ⟨.node _ ``«I» _⟩ => shape% 'I'
+| turn% ⟨.node _ ``«J» _⟩ => shape% 'J'
+| turn% ⟨.node _ ``«K» _⟩ => shape% 'K'
+| turn% ⟨.node _ ``«L» _⟩ => shape% 'L'
+| turn% ⟨.node _ ``«M» _⟩ => shape% 'M'
+| turn% ⟨.node _ ``«N» _⟩ => shape% 'N'
+| turn% ⟨.node _ ``«O» _⟩ => shape% 'O'
+| turn% ⟨.node _ ``«P» _⟩ => shape% 'P'
+| turn% ⟨.node _ ``«Q» _⟩ => shape% 'Q'
+| turn% ⟨.node _ ``«R» _⟩ => shape% 'R'
+| turn% ⟨.node _ ``«S» _⟩ => shape% 'S'
+| turn% ⟨.node _ ``«T» _⟩ => shape% 'T'
+| turn% ⟨.node _ ``«U» _⟩ => shape% 'U'
+| turn% ⟨.node _ ``«V» _⟩ => shape% 'V'
+| turn% ⟨.node _ ``«W» _⟩ => shape% 'W'
+| turn% ⟨.node _ ``«X» _⟩ => shape% 'X'
+| turn% ⟨.node _ ``«Y» _⟩ => shape% 'Y'
+| turn% ⟨.node _ ``«Z» _⟩ => shape% 'Z'
+| turn% ⟨.node _ ``lbracket _⟩ => shape% '['
+| turn% ⟨.node _ ``slash _⟩ => shape% '\\'
+| turn% ⟨.node _ ``rbracket _⟩ => shape% ']'
+| turn% ⟨.node _ ``caret _⟩ => shape% '^'
+| turn% ⟨.node _ ``underscore _⟩ => shape% '_'
+| turn% ⟨.node _ ``grave _⟩ => shape% '`'
+| turn% ⟨.node _ ``«a» _⟩ => shape% 'a'
+| turn% ⟨.node _ ``«b» _⟩ => shape% 'b'
+| turn% ⟨.node _ ``«c» _⟩ => shape% 'c'
+| turn% ⟨.node _ ``«d» _⟩ => shape% 'd'
+| turn% ⟨.node _ ``«e» _⟩ => shape% 'e'
+| turn% ⟨.node _ ``«f» _⟩ => shape% 'f'
+| turn% ⟨.node _ ``«g» _⟩ => shape% 'g'
+| turn% ⟨.node _ ``«h» _⟩ => shape% 'h'
+| turn% ⟨.node _ ``«i» _⟩ => shape% 'i'
+| turn% ⟨.node _ ``«j» _⟩ => shape% 'j'
+| turn% ⟨.node _ ``«k» _⟩ => shape% 'k'
+| turn% ⟨.node _ ``«l» _⟩ => shape% 'l'
+| turn% ⟨.node _ ``«m» _⟩ => shape% 'm'
+| turn% ⟨.node _ ``«n» _⟩ => shape% 'n'
+| turn% ⟨.node _ ``«o» _⟩ => shape% 'o'
+| turn% ⟨.node _ ``«p» _⟩ => shape% 'p'
+| turn% ⟨.node _ ``«q» _⟩ => shape% 'q'
+| turn% ⟨.node _ ``«r» _⟩ => shape% 'r'
+| turn% ⟨.node _ ``«s» _⟩ => shape% 's'
+| turn% ⟨.node _ ``«t» _⟩ => shape% 't'
+| turn% ⟨.node _ ``«u» _⟩ => shape% 'u'
+| turn% ⟨.node _ ``«v» _⟩ => shape% 'v'
+| turn% ⟨.node _ ``«w» _⟩ => shape% 'w'
+| turn% ⟨.node _ ``«x» _⟩ => shape% 'x'
+| turn% ⟨.node _ ``«y» _⟩ => shape% 'y'
+| turn% ⟨.node _ ``«z» _⟩ => shape% 'z'
+| turn% ⟨.node _ ``lbrace _⟩ => shape% '{'
+| turn% ⟨.node _ ``pipe _⟩ => shape% '|'
+| turn% ⟨.node _ ``rbrace _⟩ => shape% '}'
+| turn% ⟨.node _ ``tilde _⟩ => shape% '~'
+| spin% => some none
+| _ => none
+
+open Sodium Crypto Ethos
+
+structure _root_.IO.RealWorld.Key (τ : Sodium σ) where
+  key : Typography.Key
+  witness : Witness τ := ⟨default, fun _ => key.quantize⟩
+
+/--
+Mechanism for elaborating keypresses.
+-/
+def Typewriter (τ : Sodium σ) : PFunctor where
+  «A» := IO.RealWorld.Key τ
+  «B» | ⟨none, _⟩ => PEmpty
+      | ⟨spin%, _⟩ => Tactic
+      | ⟨turn% _, _⟩ => TermElabM Shape
+
+namespace Typewriter
+
+variable {τ : Sodium σ}
+
+instance : Coe (IO.RealWorld.Key τ) (Typewriter τ).A := ⟨id⟩
+instance : Coe (Typewriter τ).A (IO.RealWorld.Key τ) := ⟨id⟩
+
+@[simp] theorem typewriter_key_idx : (Typewriter τ).A = IO.RealWorld.Key τ := by rfl
+@[simp] theorem typewriter_norm_idx : ∀ α, (Typewriter τ).B ⟨none, α⟩ = PEmpty := by intro; rfl
+@[simp] theorem typewriter_spin_idx : ∀ α (γ : Terminal), (Typewriter τ).B ⟨some (.inr γ), α⟩ = Tactic := by intros; rfl
+@[simp] theorem typewriter_turn_idx : ∀ α (γ : Grapheme), (Typewriter τ).B ⟨turn% γ, α⟩ = TermElabM Shape := by intros; rfl
+
+instance : Inhabited (Typewriter τ).A := ⟨⟨default, default⟩⟩
+instance {α} : Inhabited (Typewriter τ α) := ⟨⟨none, default⟩, PEmpty.elim⟩
+
+protected def map {α β} := @PFunctor.map α β (Typewriter τ)
+
+def enter (γ : String) (on : String := ";") (action : IO Unit := IO.eprint "\n") : Tactic
+| `(tactic|leader% $δ) => do
+  unless γ.endsWith ⟨[← parse δ]⟩ do throwAbortTactic
+  action
+| `(tactic|done%) => do
+  let γ := γ.dropRightWhile (· = ' ')
+  unless γ.endsWith on do throwAbortTactic
+  action
+| _ => throwUnsupportedSyntax
+
+/--
+Given a `TermElabM Shape`, attempt to resolve ⊢ `ULift Char`.
+-/
+@[aesop unsafe 97% destruct (rule_sets := [«standard»])]
+def norm (γ : TermElabM Shape) : TacticM PUnit := do
+  match Shape.pull (← runTermElab γ) with
+  | turn% γ => evalTactic <| ← `(tactic|leader% $γ)
+  | spin% => evalTactic <| ← `(tactic|done%)
+  | _ => throwUnsupportedSyntax
+
+def write (γ : IO.RealWorld.Key τ) (δ : Tactic := enter default) : TacticM ((Typewriter τ).B γ) :=
+  match γ with
+  | ⟨turn% γ, _⟩ => return (Shape.push ∘ Key.mk) <$> parse γ
+  | ⟨spin%, _⟩ => pure δ
+  | _ => throwUnsupportedSyntax
+
+def read {γ : IO.RealWorld.Key τ} (writer : TacticM ((Typewriter τ).B γ)) : TacticM Unit := do
+  match γ with
+  | ⟨turn% _, _⟩ => norm (← writer)
+  | ⟨spin%, _⟩ => (← writer) <| ← `(tactic|done%)
+  | _ => throwUnsupportedSyntax
+
+/--
+Source `IO.RealWorld.Key τ` from stdin without buffering.
+-/
+def getKeyFromCore : CoreM (Option (IO.RealWorld.Key τ)) := do
+  let fd ← IO.getStdin
+  let mut key? : Option (IO.RealWorld.Key τ) := none
+  repeat match ← fd.read 1 with
+  | ⟨#[]⟩ => continue
+  | ⟨#[γ]⟩ => key? := some { key := Key.mk <| Char.ofUInt8 γ }; break
+  | _ => break
+  return key?
+
+/--
+Given a `Typewriter τ Tactic`, attempt to resolve ⊢ `ULift String`.
+
+Progress is echoed on stderr. Witnesses are printed to stdout.
+
+By default, keys are sourced from stdin (see `getKeyFromCore`).
+-/
+protected def observe
+  (writer : Typewriter τ Tactic)
+  (δ : String → Tactic := enter)
+  (ε : CoreM (Option (IO.RealWorld.Key τ)) := getKeyFromCore)
+  (pre : String := default)
+  (post : String := default)
+  : TacticM (Witness τ) :=
+do match writer with
+| ⟨⟨spin%, α⟩, press⟩ =>
+  let mut buf : String := pre
+  try
+    repeat match ← ε with
+    | some key =>
+      let γ ← mkFreshExprMVar (userName := `«γ») <| mkApp (mkConst ``ULift [levelZero]) (mkConst ``Char)
+      let _ ← Tactic.run γ.mvarId! <| read <| write key (δ buf)
+      let γ ← instantiateMVars γ
+      let γ ← Tactic.elabTermEnsuringType (← delab <| mkApp (mkConst ``ULift.down) γ) (mkConst ``Char)
+      let γ := String.mk [← unsafe evalExpr Char (mkConst ``Char) γ]
+      IO.eprint γ
+      buf := buf ++ γ
+    | _ => throwAbortTactic
+    return default
+  catch ex => do
+    unless isAbortTacticException ex do throw ex
+    let γ ← delab <| mkStrLit (buf ++ post)
+    let γ ← `(tactic|exact ⟨$γ⟩)
+    press evalTactic γ
+    return by refine Universal.map (bind · fun α => ?_) α; exact do
+      -- Provide a witness for `ULift String` using the computed value.
+      unless α.phase = .safe do return α
+      let γ ← Observable.new γ .global
+      γ.emit (← IO.getStdout) "$/spin"
+      return γ
+| ⟨⟨turn% γ, α⟩, press⟩ =>
+  press (Shape.push <$> do IO.eprint (← parse γ); pure (turn% γ)) <| ← `(tactic|done%)
+  return by refine Universal.map (bind · fun α => ?_) α; exact do
+    -- Provide a witness for `ULift String` by encoding the given grapheme as a Json string.
+    let γ ← Observable.new <| ← `(tactic|leader% $γ)
+    let γ ← γ.quantize (if α.phase = .norm then .down else if α.phase = .safe then .left else .right)
+    γ.emit (← IO.getStdout) "$/turn"
+    return γ
+| ⟨⟨none, α⟩, _⟩ => pure α
+
+protected def auto
+  (ictx : InputContext)
+  (writer : Typewriter τ Tactic)
+  (δ : String → Tactic := enter)
+  (pre : String := default)
+  (post : String := default)
+  : TacticM (Witness τ) :=
+do
+  let ref ← IO.mkRef ictx.input.data
+  Typewriter.observe writer δ (pre := pre) (post := post) do
+    match ← ref.get with
+    | [] => pure none
+    | ε :: δ => ref.set δ; return some { key := Key.mk ε }
+
+protected def print
+  (writer : Typewriter τ Tactic)
+  (δ : String → Tactic := enter)
+  (ε : CoreM (Option (IO.RealWorld.Key τ)) := getKeyFromCore)
+  (pre : String := default)
+  (post : String := default)
+  : TacticM String :=
+do
+  let γ ← mkFreshExprMVar (userName := `«γ») <| mkApp (mkConst ``ULift [levelZero]) (mkConst ``String)
+  let _ ← Tactic.run γ.mvarId! <| discard <| Typewriter.observe writer δ ε pre post
+  let γ ← instantiateMVars γ
+  let γ ← Tactic.elabTermEnsuringType (← delab <| mkApp (mkConst ``ULift.down) γ) (mkConst ``String)
+  unsafe evalExpr String (mkConst ``String) γ
+
+@[aesop unsafe 97% forward (rule_sets := [«cautious»])]
+protected def forward (ictx : InputContext) (writer : Typewriter τ Tactic) : Tactic :=
+  fun _ => discard <| Typewriter.auto ictx writer
+
+def _root_.IO.RealWorld.Typist (τ : Sodium σ) := Emulator σ ⊚ Typewriter τ
+def _root_.IO.RealWorld.Automaton (τ : Sodium σ) := Typewriter τ ⊚ Emulator σ
+
+end Typewriter
+
+export IO.RealWorld (Typist Automaton)
+
+end Typography
+
+export Typography (
+  Typewriter
+  Typewriter.map
+  Typewriter.observe
+  Typewriter.auto
+  Typewriter.print
+  Typewriter.forward
+  Typist
+  Automaton
+)
